src/Common/DecideableEnsembles.v
@@ -1,4 +1,4 @@
-Require Import ADTSynthesis.Common Coq.Arith.Arith Coq.Sets.Ensembles.
+Require Import ADTSynthesis.Common Coq.Arith.Arith Coq.Bool.Bool Coq.Sets.Ensembles.
 
 Class DecideableEnsemble {A} (P : Ensemble A) :=
   { dec : A -> bool;
@@ -21,4 +21,33 @@ Instance DecideableEnsemble_gt {A} (f f' : A -> nat)
 Proof.
   intros; find_if_inside; intuition.
   exfalso; eapply gt_not_le; eassumption.
+Defined.
+
+Instance DecideableEnsemble_And
+         {A : Type}
+         {P P' : Ensemble A}
+         {P_dec : DecideableEnsemble P}
+         {P'_dec : DecideableEnsemble P'}
+: DecideableEnsemble (fun a => P a /\ P' a) :=
+  {| dec a := (@dec _ _ P_dec a) && (@dec _ _  P'_dec a) |}.
+Proof.
+  intros; rewrite <- (@dec_decides_P _ P),
+          <- (@dec_decides_P _ P').
+  setoid_rewrite andb_true_iff; reflexivity.
+Defined.
+
+(* Class used to overload equality test notation (==) in queries. *)
+Class Query_eq (A : Type) :=
+      {A_eq_dec : forall a a' : A, {a = a'} + {a <> a'}}.
+
+Infix "==" := (A_eq_dec) (at level 1).
+
+Instance DecideableEnsemble_NEqDec
+         {A B : Type}
+         {b_eq_dec : Query_eq B}
+         (f f' : A -> B)
+: DecideableEnsemble (fun a : A => f a <> f' a) :=
+  {| dec a := if A_eq_dec (f a) (f' a) then false else true |}.
+Proof.
+  intros; find_if_inside; intuition.
 Defined.
